proof/jasmin_extracts/W64_SchnorrExtract.ec
@@ -430,19 +430,26 @@ module M(SC:Syscall_t) = {
     var cf:bool;
     var r:W64.t Array128.t;
     var ai:W64.t;
+    var rp:W64.t Array128.t;
+    var bp:W64.t Array64.t;
     var i:int;
     var z:W64.t;
+    bp <- witness;
     r <- witness;
+    rp <- witness;
     ai <- a.[0];
     (_zero, of_0, cf, r) <@ dmul1 (ai, b);
+    rp <- r;
+    bp <- b;
     aux <- (32 * 2);
     i <- 1;
     while (i < aux) {
       ai <- a.[i];
       z <- (W64.of_int i);
-      (_zero, of_0, cf, r) <@ dmul1acc (z, ai, b, r, _zero, of_0, cf);
+      (_zero, of_0, cf, rp) <@ dmul1acc (z, ai, bp, rp, _zero, of_0, cf);
       i <- i + 1;
     }
+    r <- rp;
     return (_zero, of_0, cf, r);
   }
   
@@ -551,10 +558,16 @@ module M(SC:Syscall_t) = {
   proc dcminusP (p:W64.t Array64.t, x:W64.t Array64.t) : W64.t Array64.t = {
     
     var z:W64.t Array64.t;
+    var _z:W64.t Array64.t;
+    var _p:W64.t Array64.t;
     var cf:bool;
+    _p <- witness;
+    _z <- witness;
     z <- witness;
     z <@ dbn_copy (x);
-    (cf, z) <@ dbn_subc (z, p);
+    _z <- z;
+    _p <- p;
+    (cf, z) <@ dbn_subc (_z, _p);
     x <@ dbn_cmov (cf, z, x);
     return (x);
   }
@@ -653,9 +666,11 @@ module M(SC:Syscall_t) = {
   W64.t Array32.t = {
     
     var res_0:W64.t Array32.t;
+    var _a:W64.t Array64.t;
     var xr:W64.t Array128.t;
     var xrf:W64.t Array64.t;
     var xrfd:W64.t Array32.t;
+    var _b:W64.t Array32.t;
     var xrfn:W64.t Array64.t;
     var t:W64.t Array64.t;
     var pp:W64.t Array64.t;
@@ -666,6 +681,8 @@ module M(SC:Syscall_t) = {
     var  _4:bool;
     var  _5:bool;
     var  _6:bool;
+    _a <- witness;
+    _b <- witness;
     pp <- witness;
     res_0 <- witness;
     t <- witness;
@@ -673,11 +690,14 @@ module M(SC:Syscall_t) = {
     xrf <- witness;
     xrfd <- witness;
     xrfn <- witness;
-    ( _0,  _1,  _2, xr) <@ dbn_muln (a, r);
+    _a <- a;
+    ( _0,  _1,  _2, xr) <@ dbn_muln (_a, r);
     xrf <@ div2 (xr, (2 * 32));
     xrfd <@ bn_shrink (xrf);
-    ( _3,  _4,  _5, xrfn) <@ bn_muln (xrfd, p);
-    ( _6, t) <@ dbn_subc (a, xrfn);
+    _b <- xrfd;
+    ( _3,  _4,  _5, xrfn) <@ bn_muln (_b, p);
+    _a <- a;
+    ( _6, t) <@ dbn_subc (_a, xrfn);
     pp <@ bn_expand (p);
     t <@ dcminusP (pp, t);
     res_0 <@ bn_shrink (t);
@@ -699,12 +719,18 @@ module M(SC:Syscall_t) = {
   proc bn_mulm (r:W64.t Array64.t, p:W64.t Array32.t, a:W64.t Array32.t,
                 b:W64.t Array32.t) : W64.t Array32.t = {
     
+    var _a:W64.t Array32.t;
+    var _b:W64.t Array32.t;
     var _of:bool;
     var _cf:bool;
     var c:W64.t Array64.t;
     var  _0:W64.t;
+    _a <- witness;
+    _b <- witness;
     c <- witness;
-    ( _0, _of, _cf, c) <@ bn_muln (a, b);
+    _a <- a;
+    _b <- b;
+    ( _0, _of, _cf, c) <@ bn_muln (_a, _b);
     a <@ bn_breduce (r, c, p);
     return (a);
   }
